src/crypto/aes/aes-x64/proof.dfy
@@ -7,7 +7,6 @@ include "../../../arch/x64/vale64.i.dfy"
 include "../../../lib/util/dafny_wrappers.i.dfy"
 include "../ctr.s.dfy"
 include "../aes.s.dfy"
-//include "../aes_helpers.i.dfy"
 include "ctr_helpers.i.dfy"
 
 module proof {
@@ -17,95 +16,24 @@ import opened x64_def_s
 import opened types_s
 import opened dafny_wrappers_i
 import opened AESModule
-//import opened AESHelpersModule
 import opened CTRModule
 import opened CTRHelpers
 
-/*
-lemma lemma_BitwiseAdd64xy(x : uint64, y: uint64)
-    ensures  x + y < 0x1_0000_0000_0000_0000 ==> BitwiseAdd64(x, y) == x + y
-    ensures  x + y >= 0x1_0000_0000_0000_0000 ==> BitwiseAdd64(x, y) == x + y - 0x1_0000_0000_0000_0000
-    ensures  forall x:uint64 :: BitwiseAdd64(x, 0) == x;
+lemma {:timeLimitMultiplier 2} lemma_CTR_Encrypt_Upto_Done(g : G, iv : uint64, init_ctr : uint64, out_ptr : uint64, mem: Heaplets, n : uint64)
+  requires CTR_Encrypt_Req(g.inp, g.key, g.alg);
+  requires |g.inp| == |g.outp|;
+  requires n < |g.inp|;
+  requires n < |g.outp|;
+  requires |g.inp| < 0x1_0000_0000_0000_0000 - 1;
+  requires OutWriteable(g.inp, g.out_heap, out_ptr, mem);
+  requires CTR_Encrypt_Upto_Done(g, iv, init_ctr, out_ptr, mem, n);
+  requires |CTR_Encrypt(g.inp, g.key, g.alg, iv, init_ctr)| > n;
+  ensures  |CTR_Encrypt(g.inp, g.key, g.alg, iv, init_ctr)| == |g.outp|;
+  requires CTR_Encrypt(g.inp, g.key, g.alg, iv, init_ctr)[n] == 
+              mem[g.out_heap].quads[out_ptr + n * 16].v;
+  ensures  CTR_Encrypt_Upto_Done(g, iv, init_ctr, out_ptr, mem, n + 1);
 {
-    reveal_BitwiseAdd64();
-}
-
-lemma {:timeLimitMultiplier 6} lemma_CTR_Encrypt'_Is(inp : seq<Quadword>, key : seq<uint32>, alg : Algorithm, iv : uint64, init_ctr : uint64, n : uint64, i : nat)
-  requires CTR_Encrypt_Req(inp, key, alg);
-  requires 0 < |inp| < 0x1_0000_0000_0000_0000 - 1;
-  requires i < |inp|;
-  ensures |CTR_Encrypt'(inp, key, alg, iv, init_ctr, n)| == |inp|;
-  ensures 
-    CTR_Encrypt'(inp, key, alg, iv, init_ctr, n)[i] == 
-      QuadwordXor(inp[i], AES_Encrypt(key, ctr_n(iv, init_ctr, BitwiseAdd64(n,i)), alg));
-{
-  lemma_CTR_Encrypt'_length(inp);
-  lemma_BitwiseAdd64xy(n,1); // works but times out a lot.
-  if i == 0 {
-    assert
-      CTR_Encrypt'(inp, key, alg, iv, init_ctr, n)[0] == 
-       QuadwordXor(inp[0], AES_Encrypt(key, ctr_n(iv, init_ctr, n), alg));
-  } else {
-    lemma_CTR_Encrypt'_Is(inp[1..], key, alg, iv, init_ctr, BitwiseAdd64(n,1), i - 1);
-  }
-}
-*/
-
-lemma{:timeLimitMultiplier 6} lemma_CTR_Encrypt'_Is_QuadwordXor_AES(inp : seq<Quadword>, key : seq<uint32>, alg : Algorithm, iv : uint64, init_ctr : uint64, n : uint64) 
-  requires CTR_Encrypt_Req(inp, key, alg);
-  requires 0 < |inp| < 0x1_0000_0000_0000_0000 - 1;
-  ensures |CTR_Encrypt'(inp, key, alg, iv, init_ctr, n)| == |inp|;
-  ensures forall i : nat :: i < |inp| ==>
-   CTR_Encrypt'(inp, key, alg, iv, init_ctr, n)[i] == 
-    QuadwordXor(inp[i], AES_Encrypt(key, ctr_n(iv, init_ctr, BitwiseAdd64(n,i)), alg));
-{
-  lemma_CTR_Encrypt'_length(inp);
-  lemma_BitwiseAdd64(); // works but times out a lot.
-  //lemma_BitwiseAdd64xy(n,i);
-  //lemma_BitwiseAdd64xy(n,1);
-  if |inp| == 1 {
-    assert
-      CTR_Encrypt'(inp, key, alg, iv, init_ctr, n)[0] == 
-       QuadwordXor(inp[0], AES_Encrypt(key, ctr_n(iv, init_ctr, n), alg));
-  } else {
-    lemma_CTR_Encrypt'_Is_QuadwordXor_AES(inp[1..], key, alg, iv, init_ctr, BitwiseAdd64(n,1));
-  }
-}
-
-lemma{:timeLimitMultiplier 6} lemma_CTR_Encrypt_Is_Encrypt'_zero(inp : seq<Quadword>, key : seq<uint32>, alg : Algorithm, iv : uint64, init_ctr : uint64) 
-  requires CTR_Encrypt_Req(inp, key, alg);
-  requires 0 < |inp| < 0x1_0000_0000_0000_0000 - 1;
-  ensures |CTR_Encrypt(inp, key, alg, iv, init_ctr)| == |inp|;
-  ensures CTR_Encrypt(inp, key, alg, iv, init_ctr) == CTR_Encrypt'(inp, key, alg, iv, init_ctr, 0);
-{
-  lemma_CTR_Encrypt_length(inp);
-}
-
-lemma{:timeLimitMultiplier 6} lemma_CTR_Encrypt_Is_Encrypt'_zero_gen(inp : seq<Quadword>, key : seq<uint32>, alg : Algorithm, iv : uint64, init_ctr : uint64) 
-  requires CTR_Encrypt_Req(inp, key, alg);
-  requires 0 < |inp| < 0x1_0000_0000_0000_0000 - 1;
-  ensures |CTR_Encrypt(inp, key, alg, iv, init_ctr)| == |inp|;
-  ensures forall i : nat :: i < |inp| ==> 
-    CTR_Encrypt(inp, key, alg, iv, init_ctr)[i] == CTR_Encrypt'(inp, key, alg, iv, init_ctr, 0)[i];
-{
-  lemma_CTR_Encrypt_length(inp);
-  lemma_CTR_Encrypt_Is_Encrypt'_zero(inp, key, alg, iv, init_ctr);
-}
-
-lemma{:timeLimitMultiplier 6} lemma_CTR_Encrypt_Is_QuadwordXor_AES(inp : seq<Quadword>, key : seq<uint32>, alg : Algorithm, iv : uint64, init_ctr : uint64, n : uint64)
-  requires CTR_Encrypt_Req(inp, key, alg);
-  requires 0 < |inp| < 0x1_0000_0000_0000_0000 - 1;
-  ensures |CTR_Encrypt(inp, key, alg, iv, init_ctr)| == |inp|;
-  ensures forall i : nat :: i < |inp| ==>
-   CTR_Encrypt(inp, key, alg, iv, init_ctr)[i] == 
-    QuadwordXor(inp[i], AES_Encrypt(key, ctr_n(iv, init_ctr, BitwiseAdd64(n,i)), alg));
-{
-  lemma_CTR_Encrypt'_length(inp);
-  lemma_BitwiseAdd64(); // works but times out a lot.
-
- lemma_CTR_Encrypt'_Is_QuadwordXor_AES(inp, key, alg, iv, init_ctr, n);
- lemma_CTR_Encrypt_Is_Encrypt'_zero(inp, key, alg, iv, init_ctr);
-// lemma_CTR_Encrypt_Is_Encrypt'_zero_gen(inp, key, alg, iv, init_ctr);
+  lemma_CTR_Encrypt_length'(g.inp, g.key, g.alg, iv, init_ctr);
 }
 
 }
