src/crypto/aes/gcm2.s.dfy
@@ -1,0 +1,123 @@
+include "aes.s.dfy"
+
+// Derived from NIST Special Publication 800-38D
+// http://nvlpubs.nist.gov/nistpubs/Legacy/SP/nistspecialpublication800-38d.pdf
+
+module GCM {
+
+import opened AESModule
+
+// 6.2 
+// This is specified big endian, thank gosh.
+function inc32(iv96ctr32 : Quadword) : Quadword
+{
+  reveal_BitwiseAdd32();
+  iv96ctr32.(lo := BitwiseAdd32(iv96ctr32.lo,1));
+}
+
+// 6.3 block multiply 
+
+function {:axiom} QuadwordShr(w : Quadword) : Quadword;
+function {:axiom} LEBit(w : Quadword) : bool;
+
+var R := Quadword(0b11100001000000000000000000000000, 0, 0, 0);
+
+function BlockMul(X : Quadword, Y : Quadword) {
+  var Z := Quadword(0,0,0,0);
+  var V := Y;
+  var i = 0;
+  while (i < 128) {
+    if (LEBit(X,i)) {
+      Z := QuadwordXor(Z,V);
+    } else {
+      Z := Z;
+    };
+    if (LEBit(V,0)) {
+      V := QuadwordXor(QuadwordShr(V,1), R);
+    } else {
+      V := QuadwordShr(V,1);
+    }
+  }
+  return Z;
+}
+
+function GHASH(H:Quadword, X:seq<Quadword>) : Quadword
+    requires |X| > 0;
+{
+    if |X| == 1 then
+        var Y_0 := Quadword(0, 0, 0, 0);
+        BlockMul(QuadwordXor(Y_0, X[0]), H)
+    else
+        var Y_i_minus_1 := GHASH(H, all_but_last(X));
+        BlockMul(QuadwordXor(Y_i_minus_1, last(X)), H)
+}
+
+// 6.5 GCTR 
+// We count by 0 here instead of by 1 in the spec.
+
+function CB(i : nat, ICB : Quadword) : Quadword
+{
+    if i = 0 then ICB else inc32(CB(i-1, ICB))
+}
+
+function ctr_n(ICB : Quadword, n : uint32) : Quadword 
+{
+  reveal_BitwiseAdd32();
+  Quadword(BitwiseAdd32(ICB.lo, n),
+          ICB.mid_lo,
+          ICB.mid_hi,
+          ICB.hi);
+}
+
+lemma CB_ctr_n_equivalent(ICB : Quadword, n : nat)
+  requires n < 0x1_0000_0000;
+  ensures CB(ICB,n) == ctr_n(ICB,n);
+{
+}
+
+// Algorithm 3 
+
+function AES_GCTR(key : seq<uint32>, CB : Quadword, X : seq<Quadword>) : seq<Quadword>
+    decreases |X|;
+    requires  |X| < 0x1_0000_0000 - 1;
+    ensures   |AES_GCTR( key, CB, X)| = |X|;
+{
+   if |X| == 1 then
+    [QuadwordXor(X[0], AES_Encrypt(key, ctr_n(CB, 0), AES_128))]
+   else 
+      var rest := CTR_Encrypt(key, CB, all_but_last(X));
+      rest + [QuadwordXor(X[|X| - 1], AES_Encrypt(key, ctr_n(CB, |X| - 1), AES_128))]
+}
+
+// Algorithm 4 
+// From 8.3 
+// The  total  number  of  invocations  of  the  authenticated  encryption  function  shall  not  exceed  
+// 2^32, including all IV lengths and all instances of the authenticated encryption function with 
+// the given key. 
+// So how do I get the lengths?
+//
+// This is currently fixed to an IV of 96 bits in the high bits of the IV.
+
+function AES_GCTR_AE(key : seq<uint32>, IV : Quadword, P : seq<Quadword>, A : seq<Quadword>) : (seq<Quadword>, Quadword)
+{
+    var H := AES_Encrypt(key, Quadword(0, 0, 0, 0), AES_128);
+    var J_0 := IV.(lo := 1);        // Consider the top 96 bits of the IV quadword to be the "real" IV
+    var C := AES_GCTR(key, inc32(J_0), P);
+    var lengths := Quadword(|C|*128, 0, |A|*128, 0);
+    var S := GHASH(H, additional_data + C + [lengths]);
+    var T := AES_GCTR(key, J_0, [S])[0];
+    (C, T)
+}
+
+// Algorithm 5
+
+function AES_GCTR_AD(key : seq<uint32>, IV : Quadword, C : seq<Quadword>, T: Quadword) : (seq<Quadword>, bool)
+{
+    var H := AES_Encrypt(key, Quadword(0, 0, 0, 0), AES_128);
+    var J_0 := IV.(lo := 1);        // Consider the top 96 bits of the IV quadword to be the "real" IV
+    var P := AES_GCTR(key, inc32(J_0), C);
+    var lengths := Quadword(|C|*128, 0, |A|*128, 0);
+    var S := GHASH(H, additional_data + C + [lengths]);
+    var T' := AES_GCTR(key, J_0, [S])[0];
+    (P, T == T')
+}
